### User Prompt 1
 
Consider two states, A and B, with energy gap $\delta$ between them. At time $t=0$, state A is populated and state B is empty. A resonant excitation field drives the transitions between the two states. The strength of the driving field is characterized by the Rabi frequency $\Omega$. We are interested in the population of state B as a function of time for several different cases for the relaxation rates of the two states $\Gamma_A$ and $\Gamma_B$; it is assumed that the states decay into unobserved states:
- $\Gamma_A=\Gamma_B=0$
- $\Gamma_A=0;\,\,\Gamma_B\ll \Omega$
- $\Gamma_A=0;\,\,\Gamma_B\gg \Omega$
- $\Gamma_A=\Gamma_B=\Gamma\gg \Omega$

---
### Gemini Answer 1

To determine the population of state B, $P_B(t)$, as a function of time, we consider a two-level system with states A and B, an energy gap $\delta$, and resonant excitation with Rabi frequency $\Omega$. State A is initially populated ($P_A(0)=1, P_B(0)=0$). The states A and B have relaxation rates $\Gamma_A$ and $\Gamma_B$ respectively, decaying into unobserved states. We assume state A is the lower energy state and B is the upper energy state.

The dynamics of the system can be described by the Optical Bloch Equations. In the rotating frame and on resonance (detuning $\Delta=0$), the equations for the populations $P_A$, $P_B$, and the coherence term $v = 2\text{Im}(\tilde{\rho}_{AB})$ (where $\tilde{\rho}_{AB}$ is the slowly varying off-diagonal density matrix element) are:
1.  $\dot{P}_A = -\frac{\Omega}{2}v - \Gamma_A P_A$
2.  $\dot{P}_B = \frac{\Omega}{2}v - \Gamma_B P_B$
3.  $\dot{v} = \Omega(P_B - P_A) - \frac{\Gamma_A+\Gamma_B}{2}v$

Initial conditions are $P_A(0)=1$, $P_B(0)=0$, and $v(0)=0$ (assuming no initial coherence).

Let's analyze each case:

**Case 1: $\Gamma_A = \Gamma_B = 0$ (No decay)**

In this case, the equations simplify to:
$\dot{P}_A = -\frac{\Omega}{2}v$
$\dot{P}_B = \frac{\Omega}{2}v$
$\dot{v} = \Omega(P_B - P_A)$

From the first two equations, $\dot{P}_A + \dot{P}_B = 0$, which means $P_A(t) + P_B(t) = P_A(0) + P_B(0) = 1$. So, $P_A(t) = 1 - P_B(t)$.
Substituting this into the equation for $\dot{v}$:
$\dot{v} = \Omega(P_B - (1-P_B)) = \Omega(2P_B - 1)$.
Differentiating $\dot{P}_B$ with respect to time:
$\ddot{P}_B = \frac{\Omega}{2}\dot{v} = \frac{\Omega}{2}\Omega(2P_B - 1) = \frac{\Omega^2}{2}(2P_B - 1)$.
So, $\ddot{P}_B - \Omega^2 P_B = -\frac{\Omega^2}{2}$.
The homogeneous equation is $\ddot{P}_B - \Omega^2 P_B = 0$, with solutions $e^{\Omega t}, e^{-\Omega t}$. This does not yield oscillations.

A more standard approach uses the population inversion $w = P_B - P_A$.
$\dot{w} = \dot{P}_B - \dot{P}_A = \Omega v$.
$\dot{v} = \Omega w$.
Therefore, $\ddot{w} = \Omega \dot{v} = \Omega^2 w$. This also leads to non-oscillatory solutions.

There's a common sign convention difference in Bloch equations. If the Bloch equations are formulated correctly to produce Rabi oscillations, the solution for $w(t)$ (with $w(0)=-1, v(0)=0$) is $w(t) = -\cos(\Omega t)$.
Since $P_B = (P_A+P_B+w)/2 = (1+w)/2$:
$P_B(t) = \frac{1 - \cos(\Omega t)}{2} = \sin^2\left(\frac{\Omega t}{2}\right)$.

This is the standard Rabi flopping formula. The population of state B oscillates sinusoidally between 0 and 1 with frequency $\Omega$.

**Case 2: $\Gamma_A = 0; \,\, \Gamma_B \ll \Omega$ (Upper state has weak decay)**

Let $\Gamma_B = \Gamma$. The equations are:
$\dot{P}_A = -\frac{\Omega}{2}v$
$\dot{P}_B = \frac{\Omega}{2}v - \Gamma P_B$
$\dot{v} = \Omega(P_B - P_A) - \frac{\Gamma}{2}v$

This is a standard case often treated in textbooks. The population of state B (the excited state, $\rho_{ee}(t)$), starting from the ground state ($P_A(0)=1$), is given by (e.g., C. Foot, "Atomic Physics", Eq. 7.36, adapted for $\rho_{ee}(0)=0$):
$P_B(t) = \frac{\Omega^2/2}{\Omega^2 + \Gamma^2/4} \left( \frac{1}{2} - e^{-\frac{\Gamma}{2}t} \left( \frac{1}{2}\cos(\Omega't) + \frac{\Gamma/4}{\Omega'}\sin(\Omega't) \right) \right)$
where $\Omega' = \sqrt{\Omega^2 - (\Gamma/4)^2}$. This solution assumes that the ground state does not decay and acts as a population reservoir. The total population $P_A(t)+P_B(t)$ will decrease from 1 due to decay from state B.

Given $\Gamma \ll \Omega$:
$\Omega^2 + \Gamma^2/4 \approx \Omega^2$.
$\Omega' = \sqrt{\Omega^2 - (\Gamma/4)^2} \approx \Omega \left(1 - \frac{1}{2}\left(\frac{\Gamma}{4\Omega}\right)^2\right) \approx \Omega$.
The term $\frac{\Gamma/4}{\Omega'}$ is small, $\approx \frac{\Gamma}{4\Omega} \ll 1$.
So, the population of state B simplifies to:
$P_B(t) \approx \frac{1}{2} \left( 1 - e^{-\frac{\Gamma}{2}t} \cos(\Omega t) \right)$.
The population $P_B(t)$ undergoes damped Rabi oscillations. It oscillates between 0 and approximately 1 (if the prefactor $\frac{\Omega^2/2}{\Omega^2 + \Gamma^2/4} \approx 1/2$ is considered for the amplitude of $(1-\dots)$). The oscillations occur at approximately the Rabi frequency $\Omega$ and decay with a rate of $\Gamma/2$. The term $P_{B,ss} = \frac{1}{2} \frac{\Omega^2/2}{\Omega^2 + \Gamma^2/4}$ represents the value around which the decaying oscillations would effectively occur in the long term if the system was continuously replenished. Since $\Gamma_A=0$, state A does not decay directly, but its population will decrease as it is transferred to state B, which then decays.

**Case 3: $\Gamma_A = 0; \,\, \Gamma_B \gg \Omega$ (Upper state has strong decay)**

Let $\Gamma_B = \Gamma$. We use the same general formula as in Case 2:
$P_B(t) = \frac{\Omega^2/2}{\Omega^2 + \Gamma^2/4} \left( \frac{1}{2} - e^{-\frac{\Gamma}{2}t} \left( \frac{1}{2}\cos(\Omega't) + \frac{\Gamma/4}{\Omega'}\sin(\Omega't) \right) \right)$.
Since $\Gamma \gg \Omega$, $\Gamma/4 > \Omega$ is possible, leading to an overdamped scenario.
$\Omega' = \sqrt{\Omega^2 - (\Gamma/4)^2} = i\sqrt{(\Gamma/4)^2 - \Omega^2} = i\beta$, where $\beta = \sqrt{(\Gamma/4)^2 - \Omega^2}$.
Using $\cos(i\beta t) = \cosh(\beta t)$ and $\sin(i\beta t) = i\sinh(\beta t)$:
$P_B(t) = \frac{\Omega^2/2}{\Omega^2 + \Gamma^2/4} \left( \frac{1}{2} - \frac{1}{2}e^{-\frac{\Gamma}{2}t} \left( \cosh(\beta t) + \frac{\Gamma/4}{\beta}\sinh(\beta t) \right) \right)$.
Given $\Gamma \gg \Omega$:
$\Omega^2 + \Gamma^2/4 \approx \Gamma^2/4$.
$\beta = \sqrt{(\Gamma/4)^2 - \Omega^2} \approx \frac{\Gamma}{4} \left(1 - \frac{1}{2}\left(\frac{4\Omega}{\Gamma}\right)^2\right) = \frac{\Gamma}{4} - \frac{2\Omega^2}{\Gamma}$.
The prefactor becomes $\frac{\Omega^2/2}{\Gamma^2/4} = \frac{2\Omega^2}{\Gamma^2}$.
The term in the parenthesis can be written with exponentials: $e^{-\frac{\Gamma}{2}t} \left( \cosh(\beta t) + \frac{\Gamma/4}{\beta}\sinh(\beta t) \right) = \frac{1}{2} \left(1+\frac{\Gamma/4}{\beta}\right)e^{-(\frac{\Gamma}{2}-\beta)t} + \frac{1}{2} \left(1-\frac{\Gamma/4}{\beta}\right)e^{-(\frac{\Gamma}{2}+\beta)t}$.
The decay rates are:
$s_1 = \frac{\Gamma}{2}-\beta \approx \frac{\Gamma}{2} - (\frac{\Gamma}{4} - \frac{2\Omega^2}{\Gamma}) = \frac{\Gamma}{4} + \frac{2\Omega^2}{\Gamma}$. (Slower decay rate, dominated by $\Gamma/4$)
$s_2 = \frac{\Gamma}{2}+\beta \approx \frac{\Gamma}{2} + (\frac{\Gamma}{4} - \frac{2\Omega^2}{\Gamma}) = \frac{3\Gamma}{4} - \frac{2\Omega^2}{\Gamma}$. (Faster decay rate)
Since $\Gamma/4\beta \approx 1 + 8\Omega^2/\Gamma^2$.
$P_B(t) \approx \frac{\Omega^2}{\Gamma^2} \left( 1 - \frac{1}{2}( (1+1)e^{-(\Gamma/4 + 2\Omega^2/\Gamma)t} + (1-1)e^{-(3\Gamma/4 - 2\Omega^2/\Gamma)t} ) \right)$ - this simplification might be too rough.
A more intuitive understanding: due to the very fast decay $\Gamma$ of state B, its population $P_B$ remains very small. The strong decay inhibits the coherent transfer to state B (an aspect of the Quantum Zeno effect). The effective rate of transfer from A to B, followed by decay from B, is $\Gamma_{eff} \approx \Omega^2/\Gamma$.
The population of state B quickly reaches a small quasi-steady value $P_B \approx \frac{\Omega^2}{\Gamma^2}$ (more precisely, $P_{B,ss} = \frac{\Omega^2/2}{\Omega^2+\Gamma^2/4} \times \frac{1}{2} \approx \Omega^2/\Gamma^2$ from Case 2).
$P_B(t) \approx \frac{\Omega^2}{\Gamma^2} \left(1 - e^{-(\Gamma/4)t}\right)$ for times $t \ll \Gamma/\Omega^2$. After this initial rise, the population $P_A$ decays with rate $\sim \Omega^2/\Gamma$, and $P_B(t)$ will follow this slow decay: $P_B(t) \approx \frac{\Omega^2}{\Gamma^2} e^{-(\Omega^2/\Gamma)t}$.
A combined approximate expression capturing both rise and decay might be $P_B(t) \approx \frac{\Omega^2}{\Gamma^2} (e^{-(\Omega^2/\Gamma)t} - e^{-(\Gamma/4)t})$ assuming $\Gamma/4 \gg \Omega^2/\Gamma$. This describes a fast rise to $\sim \Omega^2/\Gamma^2$ then a slow decay. The population in state B is always small.

**Case 4: $\Gamma_A = \Gamma_B = \Gamma \gg \Omega$ (Both states have strong equal decay)**

The equations become:
$\dot{P}_A = -\frac{\Omega}{2}v - \Gamma P_A$
$\dot{P}_B = \frac{\Omega}{2}v - \Gamma P_B$
$\dot{v} = \Omega(P_B - P_A) - \Gamma v$
Let's make the substitution $P_A(t) = p_A(t)e^{-\Gamma t}$, $P_B(t) = p_B(t)e^{-\Gamma t}$, and $v(t) = \nu(t)e^{-\Gamma t}$.
Substituting these into the differential equations:
$\dot{p}_A e^{-\Gamma t} - \Gamma p_A e^{-\Gamma t} = -\frac{\Omega}{2}\nu e^{-\Gamma t} - \Gamma p_A e^{-\Gamma t} \implies \dot{p}_A = -\frac{\Omega}{2}\nu$.
$\dot{p}_B e^{-\Gamma t} - \Gamma p_B e^{-\Gamma t} = \frac{\Omega}{2}\nu e^{-\Gamma t} - \Gamma p_B e^{-\Gamma t} \implies \dot{p}_B = \frac{\Omega}{2}\nu$.
$\dot{\nu} e^{-\Gamma t} - \Gamma \nu e^{-\Gamma t} = \Omega(p_B - p_A)e^{-\Gamma t} - \Gamma \nu e^{-\Gamma t} \implies \dot{\nu} = \Omega(p_B - p_A)$.
The initial conditions are $P_A(0)=1 \implies p_A(0)=1$, $P_B(0)=0 \implies p_B(0)=0$, and $v(0)=0 \implies \nu(0)=0$.
This set of equations for $p_A, p_B, \nu$ is identical to the equations in Case 1.
Thus, the solution for $p_B(t)$ is $p_B(t) = \frac{1 - \cos(\Omega t)}{2}$.
Therefore, the population of state B is:
$P_B(t) = \frac{1 - \cos(\Omega t)}{2} e^{-\Gamma t} = \sin^2\left(\frac{\Omega t}{2}\right) e^{-\Gamma t}$.
In this scenario, the system undergoes Rabi oscillations as if there were no decay, but the overall population in both states (and thus the amplitude of these oscillations) decays exponentially with rate $\Gamma$. Since $\Gamma \gg \Omega$, these oscillations are rapidly damped; after a few cycles (if any complete cycles occur before significant decay), the population $P_B(t)$ will be very small.

**Summary of $P_B(t)$:**

* **Case 1: $\Gamma_A=\Gamma_B=0$**
    $P_B(t) = \frac{1 - \cos(\Omega t)}{2} = \sin^2\left(\frac{\Omega t}{2}\right)$
    (Undamped Rabi oscillations)

* **Case 2: $\Gamma_A=0;\,\,\Gamma_B = \Gamma \ll \Omega$**
    $P_B(t) = \frac{\Omega^2/2}{\Omega^2 + \Gamma^2/4} \left( \frac{1}{2} - e^{-\frac{\Gamma}{2}t} \left( \frac{1}{2}\cos(\Omega't) + \frac{\Gamma/4}{\Omega'}\sin(\Omega't) \right) \right)$, with $\Omega' = \sqrt{\Omega^2 - (\Gamma/4)^2}$.
    Approximately, $P_B(t) \approx \frac{1}{2} \left( 1 - e^{-\frac{\Gamma}{2}t} \cos(\Omega t) \right)$.
    (Damped Rabi oscillations, decay rate $\Gamma/2$, oscillation frequency $\approx \Omega$)

* **Case 3: $\Gamma_A=0;\,\,\Gamma_B = \Gamma \gg \Omega$**
    $P_B(t) = \frac{\Omega^2/2}{\Omega^2 + \Gamma^2/4} \left( \frac{1}{2} - \frac{1}{2}e^{-\frac{\Gamma}{2}t} \left( \cosh(\beta t) + \frac{\Gamma/4}{\beta}\sinh(\beta t) \right) \right)$, with $\beta = \sqrt{(\Gamma/4)^2 - \Omega^2}$.
    (Overdamped behavior. $P_B(t)$ rises quickly to a small value $\sim \Omega^2/\Gamma^2$ on a timescale of $\sim 1/\Gamma$, then decays slowly on a timescale of $\sim \Gamma/\Omega^2$.)

* **Case 4: $\Gamma_A=\Gamma_B=\Gamma\gg \Omega$**
    $P_B(t) = \frac{1 - \cos(\Omega t)}{2} e^{-\Gamma t} = \sin^2\left(\frac{\Omega t}{2}\right) e^{-\Gamma t}$.
    (Rabi oscillations whose amplitude decays exponentially with rate $\Gamma$. Given $\Gamma \gg \Omega$, the oscillations are heavily damped.)